added expression interpreter

PyLevelLang/src/PyLevelLang/Interpret.v
@@ -1,5 +1,8 @@
 Require Import PyLevelLang.Language.
 Require Import coqutil.Map.Interface.
+Require Import PyLevelLang.Elaborate.
+
+Local Open Scope Z_scope.
 
 Fixpoint interp_type (t : type) :=
   match t with
@@ -13,7 +16,7 @@ Fixpoint interp_type (t : type) :=
 
 Fixpoint default_val (t : type) : interp_type t :=
   match t as t' return interp_type t' with
-  | TInt => 0%Z
+  | TInt => 0
   | TBool => false
   | TString => EmptyString
   | TPair t1 t2 => (default_val t1, default_val t2)
@@ -21,6 +24,110 @@ Fixpoint default_val (t : type) : interp_type t :=
   | TEmpty => tt
   end.
 
+Fixpoint eval_range (lo : Z) (len : nat) : list Z :=
+  match len with
+  | 0%nat => nil
+  | S n => lo :: eval_range (lo + 1) n
+  end.
+
+Definition proj_expected (t_expected : type) (v : {t_actual & interp_type t_actual}) : 
+  interp_type t_expected :=
+  match type_eq_dec (projT1 v) t_expected with
+  | left H => cast H _ (projT2 v)
+  | _ => default_val t_expected
+  end.
+
+Definition compare_values {t : type} : interp_type t -> interp_type t -> bool :=
+  match t with
+  | TInt => Z.eqb
+  | TString => String.eqb
+  | TBool => Bool.eqb
+  | _ => fun _ _ => false
+  end.
+
 Section WithMap.
   Context {locals: map.map string {t & interp_type t}} {locals_ok: map.ok locals}.
+
+  Fixpoint interp_expr (l : locals) {t : type} (e : expr t) : interp_type t :=
+    match e in (expr t0) return (interp_type t0) with
+    | EVar _ x => match map.get l x with
+                  | None => default_val _
+                  | Some v => proj_expected _ v
+                  end
+    | ELoc _ x => match map.get l x with
+                  | None => default_val _
+                  | Some v => proj_expected _ v
+                  end
+    | EConst c => match c with
+                  | CInt n => n
+                  | CBool b => b
+                  | CString s => s
+                  | CNil t => nil
+                  end
+    | EUnop o e1 => match o in unop t1 t2 return expr t1 -> interp_type t2 with
+                    | ONeg => fun e1 => - (interp_expr l e1)
+                    | ONot => fun e1 => negb (interp_expr l e1)
+                    | OLength _ => fun e1 => Z.of_nat (length (interp_expr l e1))
+                    | OLengthString => fun e1 => Z.of_nat (String.length (interp_expr l e1))
+                    | OFst _ _ => fun e1 => fst (interp_expr l e1)
+                    | OSnd _ _ => fun e1 => snd (interp_expr l e1)
+                    end e1
+    | EBinop o e1 e2 => match o in binop t1 t2 t3 return expr t1 -> expr t2 -> interp_type t3 with
+                        | OPlus => fun e1 e2 => interp_expr l e1 + interp_expr l e2
+                        | OMinus => fun e1 e2 => interp_expr l e1 - interp_expr l e2
+                        | OTimes => fun e1 e2 => interp_expr l e1 * interp_expr l e2
+                        | ODiv => fun e1 e2 => interp_expr l e1 / interp_expr l e2
+                        | OMod => fun e1 e2 => Zmod (interp_expr l e1) (interp_expr l e2)
+                        | OAnd => fun e1 e2 => andb (interp_expr l e1) (interp_expr l e2)
+                        | OOr => fun e1 e2 => orb (interp_expr l e1) (interp_expr l e2)
+                        | OConcat _ => fun e1 e2 => app (interp_expr l e1) (interp_expr l e2)
+                        | OConcatString => fun e1 e2 => String.append (interp_expr l e1) (interp_expr l e2)
+                        | OLess => fun e1 e2 => (interp_expr l e1) <? (interp_expr l e2)
+                        | OEq _ => fun e1 e2 => compare_values (interp_expr l e1) (interp_expr l e2)
+                        | ORepeat _ => fun e1 e2 => repeat (interp_expr l e2) (Z.to_nat (interp_expr l e1))
+                        | OPair _ _ => fun e1 e2 => (interp_expr l e1, interp_expr l e2)
+                        | OCons _ => fun e1 e2 => interp_expr l e1 :: interp_expr l e2
+                        | ORange => fun e1 e2 => 
+                            let lo := interp_expr l e1 in 
+                            let hi := interp_expr l e2 in 
+                            eval_range lo (Z.to_nat (hi - lo))
+                        end e1 e2
+    | EFlatmap e1 x e2 => 
+        flat_map (fun y => interp_expr (map.put l x (existT _ _ y)) e1) 
+        (interp_expr l e2)
+    | EIf e1 e2 e3 => match interp_expr l e1 with
+                      | true => interp_expr l e2
+                      | false => interp_expr l e3
+                      end
+    | ELet x e1 e2 => 
+        interp_expr (map.put l x (existT _ _ (interp_expr l e1))) e2
+    end.
+
 End WithMap.
+
+Section Examples.
+  Instance locals : map.map string {t & interp_type t} := SortedListString.map _.
+  Instance locals_ok : map.ok locals := SortedListString.ok _.
+
+  Definition ex1 : expr (TList TInt) :=
+      (EBinop (OCons _) (EConst (CInt 1))
+        (EBinop (OCons _) (EConst (CInt 2))
+          (EBinop (OCons _) (EConst (CInt 3))
+            (EBinop (OCons _) (EConst (CInt 4))
+              (EConst (CNil _)))))).
+  Goal interp_expr map.empty ex1 = 1 :: 2 :: 3 :: 4 :: nil.
+  reflexivity. Qed.
+
+  Definition ex2 : expr TInt:= 
+      (EUnop (OFst _ _) (ELet "x"
+        (EConst (CInt 42)) (EBinop (OPair _ _) (EVar TInt "x") (EVar TInt "x")))).
+  Goal interp_expr map.empty ex2 = 42.
+  reflexivity. Qed.
+
+  Local Open Scope string_scope.
+  Definition ex3 : expr (TPair TInt (TPair TBool TString)) :=
+      (EBinop (OPair _ _) (EConst (CInt 42))
+        (EBinop (OPair _ _) (EConst (CBool true)) (EConst (CString "hello")))).
+  Goal interp_expr map.empty ex3 = (42, (true, "hello")).
+  reflexivity. Qed.
+End Examples.
